Progress on concretization lemmas.

src/coq/Semantics/Denotation.v
@@ -155,8 +155,10 @@ Module Denotation (LP : LLVMParams) (MP : MemoryParams LP) (Byte : ByteModule LP
     | _             => concretize_or_pick uv True
     end.
 
+  (* Unique or the concretization fails *)
   Definition unique_prop (uv : uvalue) : Prop
-    := exists x, concretize uv x /\ forall dv, concretize uv dv -> dv = x.
+    := (exists x, concretize uv x /\ forall dv, concretize uv dv -> dv = x) \/
+         (forall dv, ~ concretize uv dv).
 
   Definition pickUnique {E : Type -> Type} `{PickE -< E} `{FailureE -< E} (uv : uvalue) : itree E dvalue
     := concretize_or_pick uv (unique_prop uv).
